Populate new pure_evalScript.sml

language/pure_evalScript.sml
@@ -21,9 +21,22 @@ End
 
 (* weak-head evalation *)
 
-Definition dest_wh_Closure_def:
+Definition dest_wh_Closure_def[simp]:
   dest_wh_Closure (wh_Closure s e) = SOME (s,e) ∧
   dest_wh_Closure _ = NONE
+End
+
+Definition get_atoms_def:
+  get_atoms [] = SOME (SOME []) ∧
+  get_atoms (v::vs) =
+    case v of
+    | wh_Diverge => NONE (* diverge *)
+    | wh_Atom a =>
+        (case get_atoms vs of
+         | NONE => NONE
+         | SOME NONE => SOME NONE
+         | SOME (SOME vs) => SOME (SOME (a::vs)))
+    | _ => SOME NONE (* error *)
 End
 
 Definition eval_wh_to_def:
@@ -40,18 +53,40 @@ Definition eval_wh_to_def:
     (if k = 0 then wh_Diverge else eval_wh_to (k − 1) (subst_funs f y)) ∧
   eval_wh_to k (Prim p xs) =
     if k = 0n then wh_Diverge else
-    case p of
-    | Cons s => wh_Constructor s xs
-    | Proj s i =>
+    let vs = MAP (eval_wh_to (k-1)) xs in
+      case p of
+      | Cons s => wh_Constructor s xs
+      | Proj s i =>
         (if LENGTH xs ≠ 1 then wh_Error else
-           case eval_wh_to (k-1) (HD xs) of
+           case HD vs of
            | wh_Constructor t ys => if t = s ∧ i < LENGTH ys
                                      then eval_wh_to (k-1) (EL i ys)
                                      else wh_Error
            | wh_Diverge => wh_Diverge
            | _ => wh_Error)
-    | Lit l => wh_Atom l
-    | _ => wh_Error (* TODO: fill in rest *)
+      | IsEq s i =>
+        (if LENGTH xs ≠ 1 then wh_Error else
+           case HD vs of
+           | wh_Constructor t ys => if t ≠ s then wh_Constructor "False" [] else
+                                    if i = LENGTH ys then wh_Constructor "True" []
+                                                     else wh_Error
+           | wh_Diverge => wh_Diverge
+           | _ => wh_Error)
+      | Lit l => (if xs = [] then wh_Atom l else wh_Error)
+      | If =>
+        (if LENGTH xs ≠ 3 then wh_Error else
+           case HD vs of
+           | wh_Constructor t ys =>
+              (if t = "True" ∧ ys = [] then EL 1 vs else
+               if t = "False" ∧ ys = [] then EL 2 vs else wh_Error)
+           | wh_Diverge => wh_Diverge
+           | _ => wh_Error)
+      | AtomOp a =>
+        (case get_atoms vs of
+         | NONE => wh_Diverge
+         | SOME NONE => wh_Error
+         | SOME (SOME as) =>
+             case config.parAtomOp a as of SOME v => wh_Atom v | NONE => wh_Error)
 Termination
   WF_REL_TAC `inv_image ($< LEX $<) (λ(k,x).(k,(exp_size x)))`
 End
@@ -63,7 +98,302 @@ Definition eval_wh_def:
     | NONE => wh_Diverge
 End
 
-(* TODO: prove clock-free equations for eval_wh *)
+Theorem eval_wh_eq_Diverge:
+  eval_wh e = wh_Diverge ⇔ ∀k. eval_wh_to k e = wh_Diverge
+Proof
+  fs [eval_wh_def] \\ DEEP_INTRO_TAC some_intro
+  \\ rw [] \\ metis_tac []
+QED
+
+Theorem eval_wh_neq_Diverge:
+  eval_wh e ≠ wh_Diverge ⇔ ∃k. eval_wh_to k e ≠ wh_Diverge
+Proof
+  fs [eval_wh_eq_Diverge]
+QED
+
+Theorem eval_wh_inc:
+  ∀m e n.
+    eval_wh_to n e ≠ wh_Diverge ∧ n ≤ m ⇒
+    eval_wh_to m e = eval_wh_to n e
+Proof
+  recInduct eval_wh_to_ind \\ rw []
+  \\ fs [eval_wh_to_def]
+  THEN1
+   (Cases_on ‘eval_wh_to n x = wh_Diverge’ \\ fs []
+    \\ first_x_assum drule_all \\ fs []
+    \\ TOP_CASE_TAC \\ PairCases_on ‘x'’ \\ fs []
+    \\ Cases_on ‘n = 0’ \\ fs [])
+  THEN1 (Cases_on ‘n = 0’ \\ fs [])
+  \\ Cases_on ‘∃s. p = Cons s’ \\ gvs []
+  THEN1 (rw [] \\ fs [])
+  \\ Cases_on ‘∃s. p = Lit s’ \\ gvs []
+  THEN1 (rw [] \\ fs [])
+  \\ Cases_on ‘∃s. p = If’ \\ gvs []
+  THEN1
+   (Cases_on ‘n = 0’ \\ fs []
+    \\ Cases_on ‘LENGTH xs = 3’ \\ fs [] \\ gvs [LENGTH_EQ_NUM_compute]
+    \\ first_assum (qspec_then ‘h’ assume_tac) \\ fs []
+    \\ ‘n-1 ≤ k-1’ by fs []
+    \\ first_x_assum (first_assum o mp_then (Pos last) mp_tac)
+    \\ Cases_on ‘eval_wh_to (n − 1) h’ \\ fs []
+    \\ first_assum (qspec_then ‘h'’ assume_tac) \\ fs []
+    \\ first_x_assum (qspec_then ‘h''’ assume_tac) \\ fs []
+    \\ ‘n-1 ≤ k-1’ by fs []
+    \\ rpt (first_x_assum (first_assum o mp_then (Pos last) mp_tac))
+    \\ rw [] \\ gvs [])
+  \\ Cases_on ‘∃s. p = AtomOp s’ \\ gvs []
+  THEN1
+   (Cases_on ‘n = 0’ \\ fs []
+    \\ rpt AP_THM_TAC \\ AP_TERM_TAC
+    \\ fs [PULL_FORALL,AND_IMP_INTRO]
+    \\ ‘n-1 ≤ k-1’ by fs []
+    \\ rpt (first_x_assum (first_assum o mp_then (Pos last) mp_tac))
+    \\ Cases_on ‘get_atoms (MAP (λa. eval_wh_to (n − 1) a) xs) = NONE’ \\ fs []
+    \\ pop_assum mp_tac \\ qid_spec_tac ‘xs’
+    \\ Induct \\ fs [] \\ rw []
+    \\ first_assum (qspec_then ‘h’ mp_tac) \\ strip_tac \\ fs []
+    \\ Cases_on ‘eval_wh_to (n − 1) h’ \\ fs [get_atoms_def]
+    \\ Cases_on ‘get_atoms (MAP (λa. eval_wh_to (n − 1) a) xs')’ \\ fs [])
+  \\ Cases_on ‘∃s i. p = Proj s i’
+  THEN1
+   (Cases_on ‘n = 0’ \\ gvs []
+    \\ Cases_on ‘LENGTH xs = 1’ \\ fs [] \\ gvs [LENGTH_EQ_NUM_compute]
+    \\ ‘n-1 ≤ k-1’ by fs []
+    \\ rpt (first_x_assum (first_assum o mp_then (Pos last) mp_tac))
+    \\ Cases_on ‘eval_wh_to (n − 1) h = wh_Diverge’ \\ fs []
+    \\ Cases_on ‘eval_wh_to (n − 1) h’ \\ fs []
+    \\ rw [] \\ fs [] \\ fs [AllCaseEqs()] \\ gvs [])
+  \\ Cases_on ‘∃s i. p = IsEq s i’
+  THEN1
+   (Cases_on ‘n = 0’ \\ gvs []
+    \\ Cases_on ‘LENGTH xs = 1’ \\ fs [] \\ gvs [LENGTH_EQ_NUM_compute]
+    \\ ‘n-1 ≤ k-1’ by fs []
+    \\ rpt (first_x_assum (first_assum o mp_then (Pos last) mp_tac))
+    \\ Cases_on ‘eval_wh_to (n − 1) h = wh_Diverge’ \\ fs [])
+  \\ Cases_on ‘p’ \\ fs []
+QED
+
+Theorem eval_wh_to_agree:
+  eval_wh_to k e ≠ wh_Diverge ∧
+  eval_wh_to x e ≠ wh_Diverge ⇒
+  eval_wh_to x e = eval_wh_to k e
+Proof
+  ‘k ≤ x ∨ x ≤ k’ by fs []
+  \\ metis_tac [eval_wh_inc]
+QED
+
+Theorem eval_wh_eq:
+  eval_wh e = v ⇔
+    if v = wh_Diverge
+    then ∀k. eval_wh_to k e = wh_Diverge
+    else ∃k. eval_wh_to k e = v
+Proof
+  rw [] THEN1 fs [eval_wh_eq_Diverge]
+  \\ eq_tac \\ rw []
+  THEN1
+   (fs [eval_wh_neq_Diverge]
+    \\ qexists_tac ‘k’ \\ fs []
+    \\ fs [eval_wh_def]
+    \\ DEEP_INTRO_TAC some_intro \\ rw []
+    \\ match_mp_tac eval_wh_to_agree \\ fs [])
+  THEN1
+   (fs [eval_wh_def]
+    \\ DEEP_INTRO_TAC some_intro \\ rw []
+    \\ match_mp_tac eval_wh_to_agree \\ fs [])
+QED
+
+Theorem eval_wh_Bottom:
+  eval_wh Bottom = wh_Diverge
+Proof
+  fs [eval_wh_eq_Diverge,Bottom_def]
+  \\ completeInduct_on ‘k’ \\ Cases_on ‘k’ \\ simp [Once eval_wh_to_def]
+  \\ fs [subst_funs_def,bind_def,FUPDATE_LIST,FLOOKUP_DEF,closed_def,subst_def]
+QED
+
+Theorem eval_wh_Var:
+  eval_wh (Var s) = wh_Error
+Proof
+  fs [eval_wh_eq,eval_wh_to_def]
+QED
+
+Theorem eval_wh_Lam:
+  eval_wh (Lam s x) = wh_Closure s x
+Proof
+  fs [eval_wh_eq,eval_wh_to_def]
+QED
+
+Theorem eval_wh_App:
+  eval_wh (App x y) =
+     let v = eval_wh x in
+       if v = wh_Diverge then wh_Diverge else
+         case dest_wh_Closure v of
+           NONE => wh_Error
+         | SOME (s,body) => eval_wh (bind s y body)
+Proof
+  fs [] \\ Cases_on ‘eval_wh x = wh_Diverge’ \\ fs []
+  THEN1 (fs [eval_wh_eq] \\ fs [eval_wh_to_def])
+  \\ Cases_on ‘eval_wh x’ \\ fs [dest_wh_Closure_def]
+  \\ TRY (fs [eval_wh_eq] \\ fs [eval_wh_to_def]
+          \\ qexists_tac ‘k’ \\ fs [dest_wh_Closure_def] \\ NO_TAC)
+  \\ fs [eval_wh_eq] \\ fs [eval_wh_to_def]
+  \\ IF_CASES_TAC
+  THEN1
+   (rw [] \\ fs []
+    \\ ‘eval_wh_to k x ≠ wh_Diverge’ by fs []
+    \\ drule eval_wh_to_agree \\ pop_assum kall_tac
+    \\ disch_then drule \\ fs [dest_wh_Closure_def])
+  \\ fs []
+  \\ qexists_tac ‘k+k'+1’ \\ fs []
+  \\ ‘eval_wh_to (k+k'+1) x = eval_wh_to k x’ by (match_mp_tac eval_wh_inc \\ fs [])
+  \\ fs [dest_wh_Closure_def,PULL_EXISTS]
+  \\ qexists_tac ‘k+k'’ \\ fs []
+  \\ ‘k' ≤ k + k'’ by fs []
+  \\ metis_tac [eval_wh_inc]
+QED
+
+Theorem eval_wh_Letrec:
+  eval_wh (Letrec f y) = eval_wh (subst_funs f y)
+Proof
+  fs [Once eval_wh_eq] \\ IF_CASES_TAC
+  \\ fs [eval_wh_eq_Diverge,eval_wh_to_def]
+  \\ qexists_tac ‘k+1’ \\ fs []
+  \\ once_rewrite_tac [EQ_SYM_EQ]
+  \\ simp [eval_wh_eq] \\ qexists_tac ‘k’ \\ fs []
+QED
+
+Theorem eval_wh_Cons:
+  eval_wh (Cons s xs) = wh_Constructor s xs
+Proof
+  fs [Once eval_wh_eq,eval_wh_to_def]
+  \\ qexists_tac ‘1’ \\ fs []
+QED
+
+Theorem eval_wh_Lit:
+  eval_wh (Lit l) = wh_Atom l
+Proof
+  fs [Once eval_wh_eq,eval_wh_to_def]
+  \\ qexists_tac ‘1’ \\ fs []
+QED
+
+Theorem eval_wh_Fail:
+  eval_wh Fail = wh_Error
+Proof
+  fs [Once eval_wh_eq,eval_wh_to_def]
+  \\ qexists_tac ‘1’ \\ fs []
+QED
+
+Theorem eval_wh_If:
+  eval_wh (If x y z) =
+    if eval_wh x = wh_Diverge                then wh_Diverge else
+    if eval_wh x = wh_Constructor "True" []  then eval_wh y  else
+    if eval_wh x = wh_Constructor "False" [] then eval_wh z  else wh_Error
+Proof
+  fs [] \\ Cases_on ‘eval_wh x = wh_Diverge’ \\ fs []
+  THEN1 (fs [eval_wh_eq] \\ fs [eval_wh_to_def])
+  \\ Cases_on ‘eval_wh x’ \\ fs []
+  \\ TRY (fs [eval_wh_eq] \\ fs [eval_wh_to_def]
+          \\ qexists_tac ‘k+1’ \\ fs [] \\ NO_TAC)
+  \\ fs [eval_wh_eq] \\ fs [eval_wh_to_def]
+  \\ reverse (Cases_on ‘l=[]’) \\ gvs []
+  THEN1 (qexists_tac ‘k+1’ \\ fs [])
+  \\ Cases_on ‘s ≠ "True" ∧ s ≠ "False"’
+  THEN1 (fs [] \\ qexists_tac ‘k+1’ \\ fs [])
+  \\ gvs [] \\ rename [‘eval_wh q = wh_Diverge’]
+  \\ (Cases_on ‘eval_wh q = wh_Diverge’ \\ fs []
+      THEN1
+       (Cases \\ fs []
+        \\ Cases_on ‘eval_wh_to n x = wh_Diverge’ \\ fs []
+        \\ ‘eval_wh_to n x = eval_wh_to k x’ by (irule eval_wh_to_agree \\ fs [])
+        \\ gvs [] \\ fs [eval_wh_eq])
+      \\ fs [eval_wh_eq]
+      \\ qexists_tac ‘k+k'+1’ \\ fs []
+      \\ ‘eval_wh_to (k+k') x = eval_wh_to k x’ by (match_mp_tac eval_wh_inc \\ fs [])
+      \\ ‘eval_wh_to (k+k') q = eval_wh_to k' q’ by (match_mp_tac eval_wh_inc \\ fs [])
+      \\ fs [] \\ qexists_tac ‘k'’ \\ fs [])
+QED
+
+Theorem eval_wh_IsEq:
+  eval_wh (IsEq s i x) =
+    case eval_wh x of
+    | wh_Constructor t ys => if t ≠ s then wh_Constructor "False" []
+                             else if i = LENGTH ys then wh_Constructor "True" []
+                             else wh_Error
+    | wh_Diverge => wh_Diverge
+    | _ => wh_Error
+Proof
+  fs [] \\ Cases_on ‘eval_wh x = wh_Diverge’ \\ fs []
+  THEN1 (fs [eval_wh_eq] \\ fs [eval_wh_to_def])
+  \\ Cases_on ‘eval_wh x’ \\ fs []
+  \\ TRY (fs [eval_wh_eq] \\ fs [eval_wh_to_def]
+          \\ qexists_tac ‘k+1’ \\ fs [] \\ NO_TAC)
+  \\ fs [eval_wh_eq] \\ fs [eval_wh_to_def]
+  \\ fs [AllCaseEqs()]
+  \\ qexists_tac ‘k+1’ \\ fs []
+  \\ CCONTR_TAC \\ fs [] \\ gvs []
+QED
+
+Theorem eval_wh_Proj:
+  eval_wh (Proj s i x) =
+    case eval_wh x of
+    | wh_Constructor t ys => if t = s ∧ i < LENGTH ys
+                             then eval_wh (EL i ys) else wh_Error
+    | wh_Diverge => wh_Diverge
+    | _ => wh_Error
+Proof
+  fs [] \\ Cases_on ‘eval_wh x = wh_Diverge’ \\ fs []
+  THEN1 (fs [eval_wh_eq] \\ fs [eval_wh_to_def])
+  \\ Cases_on ‘eval_wh x’ \\ fs []
+  \\ TRY (fs [eval_wh_eq] \\ fs [eval_wh_to_def]
+          \\ qexists_tac ‘k+1’ \\ fs [] \\ NO_TAC)
+  \\ fs [eval_wh_eq] \\ fs [eval_wh_to_def]
+  \\ Cases_on ‘s ≠ s'’ \\ gvs []
+  THEN1 (qexists_tac ‘k+1’ \\ fs [])
+  \\ Cases_on ‘LENGTH l ≤ i’ \\ fs []
+  THEN1 (qexists_tac ‘k+1’ \\ fs [])
+  \\ IF_CASES_TAC
+  THEN1
+   (Cases \\ fs [GSYM NOT_LESS] \\ fs [eval_wh_eq]
+    \\ Cases_on ‘eval_wh_to n x = wh_Diverge’ \\ fs []
+    \\ ‘eval_wh_to k x = eval_wh_to n x’ by
+      (match_mp_tac eval_wh_to_agree \\ fs [])
+    \\ fs [])
+  \\ fs [eval_wh_eq]
+  \\ qexists_tac ‘k+k'+1’ \\ fs []
+  \\ ‘eval_wh_to (k + k') x = eval_wh_to k x’ by (irule eval_wh_inc \\ fs [])
+  \\ ‘eval_wh_to (k + k') (EL i l) =
+      eval_wh_to k' (EL i l)’ by (irule eval_wh_inc \\ fs [])
+  \\ fs [] \\ qexists_tac ‘k+k'’ \\ fs []
+QED
+
+Theorem eval_wh_thm:
+  eval_wh (Var s) = wh_Error ∧
+  eval_wh (Lam s x) = wh_Closure s x ∧
+  eval_wh (App x y) =
+    (let v = eval_wh x in
+       if v = wh_Diverge then wh_Diverge else
+         case dest_wh_Closure v of
+           NONE => wh_Error
+         | SOME (s,body) => eval_wh (bind s y body)) ∧
+  eval_wh (Letrec f y) = eval_wh (subst_funs f y) ∧
+  eval_wh (Cons s xs) = wh_Constructor s xs ∧
+  eval_wh (Lit l) = wh_Atom l ∧
+  eval_wh (If x y z) =
+    (if eval_wh x = wh_Diverge                then wh_Diverge else
+     if eval_wh x = wh_Constructor "True" []  then eval_wh y  else
+     if eval_wh x = wh_Constructor "False" [] then eval_wh z  else wh_Error) ∧
+  eval_wh (IsEq s i x) =
+    (case eval_wh x of
+     | wh_Constructor t ys => if t ≠ s then wh_Constructor "False" []
+                              else if i = LENGTH ys then wh_Constructor "True" []
+                              else wh_Error
+     | wh_Diverge => wh_Diverge
+     | _ => wh_Error) ∧
+  eval_wh Fail = wh_Error ∧
+  eval_wh Bottom = wh_Diverge
+Proof
+  fs [eval_wh_Lam,eval_wh_Var,eval_wh_App,eval_wh_Letrec,eval_wh_Cons,
+      eval_wh_Bottom,eval_wh_Lit,eval_wh_Fail,eval_wh_If,eval_wh_IsEq]
+QED
 
 (* unlimitied evaluation *)
 
@@ -131,6 +461,9 @@ Proof
   rw [] \\ Cases_on ‘v’ \\ gs[dest_Closure_def]
 QED
 
+Overload True  = “Constructor "True" []”;
+Overload False = “Constructor "False" []”;
+
 Definition el_def:
   el s i x =
     if x = Diverge then Diverge else
@@ -152,17 +485,117 @@ Definition is_eq_def:
       | _ => Error
 End
 
+Theorem eval_App:
+  eval (App x y) =
+    (let v = eval x in
+       if v = Diverge then Diverge else
+         case dest_Closure v of
+         | NONE => Error
+         | SOME (s,body) => eval (bind s y body))
+Proof
+  simp [eval_def,Once v_unfold,eval_wh_thm]
+  \\ once_rewrite_tac [EQ_SYM_EQ]
+  \\ simp [Once v_unfold,eval_wh_thm]
+  \\ Cases_on ‘eval_wh x’ \\ fs [dest_wh_Closure_def]
+  \\ simp [Once v_unfold,eval_wh_thm,dest_wh_Closure_def,dest_Closure_def]
+  \\ simp [Once v_unfold,eval_wh_thm,dest_wh_Closure_def,dest_Closure_def]
+QED
+
+Theorem eval_Bottom:
+  eval Bottom = Diverge
+Proof
+  simp [eval_def,Once v_unfold,eval_wh_thm]
+QED
+
+Theorem eval_Fail:
+  eval Fail = Error
+Proof
+  simp [eval_def,Once v_unfold,eval_wh_thm]
+QED
+
+Theorem eval_Var:
+  eval (Var s) = Error
+Proof
+  simp [eval_def,Once v_unfold,eval_wh_thm]
+QED
+
+Theorem eval_Cons:
+  eval (Cons s xs) = Constructor s (MAP eval xs)
+Proof
+  simp [eval_def,Once v_unfold,eval_wh_thm,MAP_EQ_f]
+QED
+
+Theorem eval_Lam:
+  eval (Lam s x) = Closure s x
+Proof
+  simp [eval_def,Once v_unfold,eval_wh_thm]
+QED
+
+Theorem eval_Letrec:
+  eval (Letrec f x) = eval (subst_funs f x)
+Proof
+  simp [eval_def,eval_wh_thm] \\ once_rewrite_tac [v_unfold] \\ fs [eval_wh_thm]
+QED
+
+Theorem eval_IsEq:
+  eval (IsEq s n x) = is_eq s n (eval x)
+Proof
+  simp [eval_def,is_eq_def]
+  \\ once_rewrite_tac [v_unfold]
+  \\ Cases_on ‘eval_wh x’ \\ fs [eval_wh_IsEq]
+  \\ rw [] \\ fs []
+QED
+
+Theorem eval_Proj:
+  eval (Proj s i x) = el s i (eval x)
+Proof
+  simp [eval_def,el_def]
+  \\ once_rewrite_tac [v_unfold]
+  \\ Cases_on ‘eval_wh x’ \\ fs [eval_wh_Proj,EL_MAP]
+  \\ Cases_on ‘s ≠ s'’ \\ gvs []
+  \\ Cases_on ‘i < LENGTH l’ \\ gvs []
+  \\ once_rewrite_tac [EQ_SYM_EQ]
+  \\ simp [Once v_unfold]
+QED
+
+Theorem eval_Lit:
+  eval (Lit l) = Atom l
+Proof
+  simp [eval_def,Once v_unfold,eval_wh_thm]
+QED
+
+Theorem eval_Let:
+  eval (Let s x y) = eval (bind s x y)
+Proof
+  fs [eval_App,eval_Lam]
+QED
+
+Theorem eval_If:
+  eval (If x y z) =
+     if eval x = Diverge then Diverge else
+     if eval x = True    then eval y  else
+     if eval x = False   then eval z  else Error
+Proof
+  simp [eval_def]
+  \\ once_rewrite_tac [v_unfold]
+  \\ Cases_on ‘eval_wh x’ \\ fs [eval_wh_If]
+  \\ Cases_on ‘l=[]’ \\ gvs []
+  \\ rw [] \\ fs []
+QED
+
 Theorem eval_thm:
-  eval (Fail)  = Error ∧
+  eval Fail = Error ∧
+  eval Bottom = Diverge ∧
   eval (Var s) = Error (* free variables are not allowed *) ∧
   eval (Cons s xs) = Constructor s (MAP eval xs) ∧
   eval (IsEq s n x) = is_eq s n (eval x) ∧
   eval (Proj s i x) = el s i (eval x) ∧
+  eval (Lit l) = Atom l ∧
   eval (Let s x y) = eval (bind s x y) ∧
-  eval (If x y z) = (
-       if eval x = Diverge then Diverge  else
-       if eval x = True    then eval y else
-       if eval x = False   then eval z else Error) ∧
+  eval (If x y z) =
+    (if eval x = Diverge then Diverge  else
+     if eval x = True    then eval y else
+     if eval x = False   then eval z else Error) ∧
   eval (Lam s x) = Closure s x ∧
   eval (Letrec f x) = eval (subst_funs f x) ∧
   eval (App x y) =
@@ -172,7 +605,8 @@ Theorem eval_thm:
          | NONE => Error
          | SOME (s,body) => eval (bind s y body))
 Proof
-  cheat (* TODO *)
+  fs [eval_App,eval_Fail,eval_Bottom,eval_Var,eval_Cons,eval_Lam,eval_Letrec,
+      eval_If,eval_Proj,eval_IsEq,eval_Lit]
 QED
 
 val _ = export_theory();
